thys/Ribbon_Proofs/Ribbons_Graphical_Soundness.thy
@@ -1,30 +1,30 @@
 section {* Soundness for graphical diagrams *}
 
-theory Ribbons_Graphical_Soundness imports 
-  Ribbons_Graphical 
+theory Ribbons_Graphical_Soundness imports
+  Ribbons_Graphical
   Finite_Map2
 begin
 
-text {* We prove that the proof rules for graphical ribbon proofs are sound 
+text {* We prove that the proof rules for graphical ribbon proofs are sound
   with respect to the rules of separation logic.
 
-  We impose an additional assumption to achieve soundness: that the 
+  We impose an additional assumption to achieve soundness: that the
   Frame rule has no side-condition. This assumption is reasonable because there
   are several separation logics that lack such a side-condition, such as
-  ``variables-as-resource''. 
+  ``variables-as-resource''.
 
-  We first describe how to extract proofchains from a diagram. This process is 
+  We first describe how to extract proofchains from a diagram. This process is
   similar to the process of extracting commands from a diagram, which was
   described in @{theory Ribbons_Graphical}. When we extract a proofchain, we
   don't just include the commands, but the assertions in between them. Our
-  main lemma for proving soundness says that each of these proofchains 
+  main lemma for proving soundness says that each of these proofchains
   corresponds to a valid separation logic proof.
 *}
 
 subsection {* Proofstate chains *}
 
-text {* When extracting a proofchain from a diagram, we need to keep track 
-  of which nodes we have processed and which ones we haven't. A 
+text {* When extracting a proofchain from a diagram, we need to keep track
+  of which nodes we have processed and which ones we haven't. A
   proofstate, defined below, maps a node to ``Top'' if it hasn't been
   processed and ``Bot'' if it has. *}
 
@@ -35,14 +35,14 @@ type_synonym proofstate = "node \<rightharpoonup>\<^sub>f topbot"
 text {* A proofstate chain contains all the nodes and edges of a graphical
   diagram, interspersed with proofstates that track which nodes have been
   processed at each point. *}
- 
+
 type_synonym ps_chain = "(proofstate, node + edge) chain"
 
 text {* The @{term "next_ps \<sigma>"} function processes one node or one edge in a
   diagram, given the current proofstate @{term \<sigma>}. It processes a node
-  @{term v} by replacing the mapping from @{term v} to @{term Top} with a 
-  mapping from @{term v} to @{term Bot}. It processes an edge @{term e} 
-  (whose source and target nodes are @{term vs} and @{term ws} respectively) 
+  @{term v} by replacing the mapping from @{term v} to @{term Top} with a
+  mapping from @{term v} to @{term Bot}. It processes an edge @{term e}
+  (whose source and target nodes are @{term vs} and @{term ws} respectively)
   by removing all the mappings from @{term vs} to @{term Bot}, and adding
   mappings from @{term ws} to @{term Top}. *}
 
@@ -51,8 +51,8 @@ where
   "next_ps \<sigma> (Inl v) = \<sigma> \<ominus> {|v|} \<oplus> [{|v|} |=> Bot]"
 | "next_ps \<sigma> (Inr e) = \<sigma> \<ominus> fst3 e \<oplus> [thd3 e |=> Top]"
 
-text {* The function @{term "mk_ps_chain \<Pi> \<pi>"} generates from @{term \<pi>}, which 
-  is a list of nodes and edges, a proofstate chain, by interspersing the 
+text {* The function @{term "mk_ps_chain \<Pi> \<pi>"} generates from @{term \<pi>}, which
+  is a list of nodes and edges, a proofstate chain, by interspersing the
   elements of @{term \<pi>} with the appropriate proofstates. The first argument
   @{term \<Pi>} is the part of the chain that has already been converted. *}
 
@@ -78,15 +78,15 @@ qed
 
 text {* Distributing @{term mk_ps_chain} over @{term Cons}. *}
 lemma mk_ps_chain_cons:
-  "mk_ps_chain \<Pi> (x # \<pi>) = mk_ps_chain (cSnoc \<Pi> x (next_ps (post \<Pi>) x)) \<pi>" 
+  "mk_ps_chain \<Pi> (x # \<pi>) = mk_ps_chain (cSnoc \<Pi> x (next_ps (post \<Pi>) x)) \<pi>"
 by (auto simp add: mk_ps_chain_def)
 
 text {* Distributing @{term mk_ps_chain} over @{term snoc}. *}
 lemma mk_ps_chain_snoc:
-  "mk_ps_chain \<Pi> (\<pi> @ [x]) 
+  "mk_ps_chain \<Pi> (\<pi> @ [x])
     = cSnoc (mk_ps_chain \<Pi> \<pi>) x (next_ps (post (mk_ps_chain \<Pi> \<pi>)) x)"
 by (unfold mk_ps_chain_def, auto)
- 
+
 text {* Distributing @{term mk_ps_chain} over @{term cCons}. *}
 lemma mk_ps_chain_ccons:
   fixes \<pi> \<Pi>
@@ -98,13 +98,13 @@ lemma pre_mk_ps_chain:
   shows "pre (mk_ps_chain \<Pi> \<pi>) = pre \<Pi>"
 apply (induct \<pi> arbitrary: \<Pi>)
 apply (auto simp add: mk_ps_chain_def mk_ps_chain_cons pre_snoc)
-done 
+done
 
 text {* A chain which is obtained from the list @{term \<pi>}, has @{term \<pi>}
   as its list of commands. The following lemma states this in a slightly
   more general form, that allows for part of the chain to have already
   been processed. *}
- 
+
 lemma comlist_mk_ps_chain:
   "comlist (mk_ps_chain \<Pi> \<pi>) = comlist \<Pi> @ \<pi>"
 proof (induct \<pi> arbitrary: \<Pi>)
@@ -112,7 +112,7 @@ proof (induct \<pi> arbitrary: \<Pi>)
   thus ?case by (auto simp add: mk_ps_chain_def)
 next
   case (Cons x \<pi>')
-  show ?case 
+  show ?case
   apply (unfold mk_ps_chain_def foldl.simps, fold mk_ps_chain_def)
   apply (auto simp add: Cons comlist_snoc)
   done
@@ -126,35 +126,35 @@ text {* In order to perform induction over our diagrams, we shall wish
   connected to that node.
 
   Hence, we consider ``partially-processed diagrams'' @{term "(G,S)"}, which
-  comprise a diagram @{term G} and a set @{term S} of nodes. @{term S} denotes 
-  the subset of @{term G}'s initial nodes that have already been processed, 
+  comprise a diagram @{term G} and a set @{term S} of nodes. @{term S} denotes
+  the subset of @{term G}'s initial nodes that have already been processed,
   and can be thought of as having been removed from @{term G}.
 
   We now give an updated version of the @{term "lins G"} function. This was
   originally defined in @{theory Ribbons_Graphical}. We provide an extra
-  parameter, @{term S}, which denotes the subset of @{term G}'s initial nodes 
+  parameter, @{term S}, which denotes the subset of @{term G}'s initial nodes
   that shouldn't be included in the linear extensions. *}
 
 definition lins2 :: "[node fset, diagram] \<Rightarrow> lin set"
 where
   "lins2 S G \<equiv> {\<pi> :: lin .
-    (distinct \<pi>) 
-  \<and> (set \<pi> = (fset G^V - fset S) <+> set G^E) 
-  \<and> (\<forall>i j v e. i < length \<pi> \<and> j < length \<pi> 
-    \<and> \<pi>!i = Inl v \<and> \<pi>!j = Inr e \<and> v |\<in>| fst3 e \<longrightarrow> i<j) 
-  \<and> (\<forall>j k w e. j < length \<pi> \<and> k < length \<pi> 
+    (distinct \<pi>)
+  \<and> (set \<pi> = (fset G^V - fset S) <+> set G^E)
+  \<and> (\<forall>i j v e. i < length \<pi> \<and> j < length \<pi>
+    \<and> \<pi>!i = Inl v \<and> \<pi>!j = Inr e \<and> v |\<in>| fst3 e \<longrightarrow> i<j)
+  \<and> (\<forall>j k w e. j < length \<pi> \<and> k < length \<pi>
     \<and> \<pi>!j = Inr e \<and> \<pi>!k = Inl w \<and> w |\<in>| thd3 e \<longrightarrow> j<k) }"
 
 lemma lins2D:
   assumes "\<pi> \<in> lins2 S G"
   shows "distinct \<pi>"
     and "set \<pi> = (fset G^V - fset S) <+> set G^E"
-    and "\<And>i j v e. \<lbrakk> i < length \<pi> ; j < length \<pi> ; 
+    and "\<And>i j v e. \<lbrakk> i < length \<pi> ; j < length \<pi> ;
       \<pi>!i = Inl v ; \<pi>!j = Inr e ; v |\<in>| fst3 e \<rbrakk> \<Longrightarrow> i<j"
     and "\<And>i k w e. \<lbrakk> j < length \<pi> ; k < length \<pi> ;
       \<pi>!j = Inr e ; \<pi>!k = Inl w ; w |\<in>| thd3 e \<rbrakk> \<Longrightarrow> j<k"
-using assms 
-apply (unfold lins2_def Collect_iff) 
+using assms
+apply (unfold lins2_def Collect_iff)
 apply (elim conjE, assumption)+
 apply blast+
 done
@@ -162,12 +162,12 @@ done
 lemma lins2I:
   assumes "distinct \<pi>"
     and "set \<pi> = (fset G^V - fset S) <+> set G^E"
-    and "\<And>i j v e. \<lbrakk> i < length \<pi> ; j < length \<pi> ; 
+    and "\<And>i j v e. \<lbrakk> i < length \<pi> ; j < length \<pi> ;
       \<pi>!i = Inl v ; \<pi>!j = Inr e ; v |\<in>| fst3 e \<rbrakk> \<Longrightarrow> i<j"
     and "\<And>j k w e. \<lbrakk> j < length \<pi> ; k < length \<pi> ;
       \<pi>!j = Inr e ; \<pi>!k = Inl w ; w |\<in>| thd3 e \<rbrakk> \<Longrightarrow> j<k"
   shows "\<pi> \<in> lins2 S G"
-using assms 
+using assms
 apply (unfold lins2_def Collect_iff, intro conjI)
 apply assumption+
 apply blast+
@@ -180,15 +180,15 @@ by (unfold lins_def lins2_def, auto)
 
 text {* The first proofstate for a diagram @{term G} is obtained by
   mapping each of its initial nodes to @{term Top}. *}
-definition 
+definition
   initial_ps :: "diagram \<Rightarrow> proofstate"
 where
   "initial_ps G \<equiv> [ initials G |=> Top ]"
 
-text {* The first proofstate for the partially-processed diagram @{term G} is 
+text {* The first proofstate for the partially-processed diagram @{term G} is
   obtained by mapping each of its initial nodes to @{term Top}, except those
   in @{term S}, which are mapped to @{term Bot}. *}
-definition 
+definition
   initial_ps2 :: "[node fset, diagram] \<Rightarrow> proofstate"
 where
   "initial_ps2 S G \<equiv> [ initials G - S |=> Top ] \<oplus> [ S |=> Bot ]"
@@ -203,17 +203,17 @@ done
 
 text {* The following function extracts the set of proofstate chains from
    a diagram. *}
-definition 
+definition
   ps_chains :: "diagram \<Rightarrow> ps_chain set"
-where 
+where
   "ps_chains G \<equiv> mk_ps_chain (cNil (initial_ps G)) ` lins G"
 
 text {* The following function extracts the set of proofstate chains from
    a partially-processed diagram. Nodes in @{term S} are excluded from
    the resulting chains. *}
-definition 
+definition
   ps_chains2 :: "[node fset, diagram] \<Rightarrow> ps_chain set"
-where 
+where
   "ps_chains2 S G \<equiv> mk_ps_chain (cNil (initial_ps2 S G)) ` lins2 S G"
 
 text {* When @{term S} is empty, the above two definitions coincide. *}
@@ -228,12 +228,12 @@ done
 
 text {* We now wish to describe proofstates chain that are well-formed. First,
   let us say that @{term "f \<oplus>disjoint g"} is defined, when @{term f} and
-  @{term g} have disjoint domains, as @{term "f \<oplus> g"}. Then, a well-formed 
-  proofstate chain consists of triples of the form @{term "(\<sigma> \<oplus>disjoint 
-  [{| v |} |=> Top], Inl v, \<sigma> \<oplus>disjoint [{| v |} |=> Bot])"}, where @{term v} 
-  is a node, or of the form @{term "(\<sigma> \<oplus>disjoint [{| vs |} |=> Bot], Inr e, 
+  @{term g} have disjoint domains, as @{term "f \<oplus> g"}. Then, a well-formed
+  proofstate chain consists of triples of the form @{term "(\<sigma> \<oplus>disjoint
+  [{| v |} |=> Top], Inl v, \<sigma> \<oplus>disjoint [{| v |} |=> Bot])"}, where @{term v}
+  is a node, or of the form @{term "(\<sigma> \<oplus>disjoint [{| vs |} |=> Bot], Inr e,
   \<sigma> \<oplus>disjoint [{| ws |} |=> Top])"}, where @{term e} is an edge with source
-  and target nodes @{term vs} and @{term ws} respectively. 
+  and target nodes @{term vs} and @{term ws} respectively.
 
   The definition below describes a well-formed triple; we then lift this
   to complete chains shortly. *}
@@ -242,24 +242,24 @@ definition
   wf_ps_triple :: "proofstate \<times> (node + edge) \<times> proofstate \<Rightarrow> bool"
 where
   "wf_ps_triple T = (case snd3 T of
-    Inl v \<Rightarrow> (\<exists>\<sigma>. v |\<notin>| fdom \<sigma> 
-      \<and> fst3 T = [ {|v|} |=> Top ] \<oplus> \<sigma> 
+    Inl v \<Rightarrow> (\<exists>\<sigma>. v |\<notin>| fdom \<sigma>
+      \<and> fst3 T = [ {|v|} |=> Top ] \<oplus> \<sigma>
       \<and> thd3 T = [ {|v|} |=> Bot ] \<oplus> \<sigma>)
-  | Inr e \<Rightarrow> (\<exists>\<sigma>. (fst3 e |\<union>| thd3 e) |\<inter>| fdom \<sigma> = {||} 
-      \<and> fst3 T = [ fst3 e |=> Bot ] \<oplus> \<sigma> 
+  | Inr e \<Rightarrow> (\<exists>\<sigma>. (fst3 e |\<union>| thd3 e) |\<inter>| fdom \<sigma> = {||}
+      \<and> fst3 T = [ fst3 e |=> Bot ] \<oplus> \<sigma>
       \<and> thd3 T = [ thd3 e |=> Top ] \<oplus> \<sigma>))"
 
 lemma wf_ps_triple_nodeI:
-  assumes "\<exists>\<sigma>. v |\<notin>| fdom \<sigma>  \<and> 
-    \<sigma>1 = [ {|v|} |=> Top ] \<oplus> \<sigma> \<and> 
+  assumes "\<exists>\<sigma>. v |\<notin>| fdom \<sigma>  \<and>
+    \<sigma>1 = [ {|v|} |=> Top ] \<oplus> \<sigma> \<and>
     \<sigma>2 = [ {|v|} |=> Bot ] \<oplus> \<sigma>"
   shows "wf_ps_triple (\<sigma>1, Inl v, \<sigma>2)"
 using assms unfolding wf_ps_triple_def
 by (auto simp add: fst3_simp snd3_simp thd3_simp)
 
 lemma wf_ps_triple_edgeI:
-  assumes "\<exists>\<sigma>. (fst3 e |\<union>| thd3 e) |\<inter>| fdom \<sigma> = {||} 
-      \<and> \<sigma>1 = [ fst3 e |=> Bot ] \<oplus> \<sigma> 
+  assumes "\<exists>\<sigma>. (fst3 e |\<union>| thd3 e) |\<inter>| fdom \<sigma> = {||}
+      \<and> \<sigma>1 = [ fst3 e |=> Bot ] \<oplus> \<sigma>
       \<and> \<sigma>2 = [ thd3 e |=> Top ] \<oplus> \<sigma>"
   shows "wf_ps_triple (\<sigma>1, Inr e, \<sigma>2)"
 using assms unfolding wf_ps_triple_def
@@ -271,7 +271,7 @@ where
   "wf_ps_chain \<equiv> chain_all wf_ps_triple"
 
 lemma next_initial_ps2_vertex:
-  "initial_ps2 ({|v|} |\<union>| S) G 
+  "initial_ps2 ({|v|} |\<union>| S) G
   = initial_ps2 S G \<ominus> {|v|} \<oplus> [ {|v|} |=> Bot ]"
 apply (unfold initial_ps2_def)
 apply transfer
@@ -279,22 +279,22 @@ apply (auto simp add: make_map_def map_diff_def map_add_def restrict_map_def)
 done
 
 lemma next_initial_ps2_edge:
-  assumes "G = Graph V \<Lambda> E" and "G' = Graph V' \<Lambda> E'" and 
-    "V' = V - fst3 e" and "E' = removeAll e E" and "e \<in> set E" and 
+  assumes "G = Graph V \<Lambda> E" and "G' = Graph V' \<Lambda> E'" and
+    "V' = V - fst3 e" and "E' = removeAll e E" and "e \<in> set E" and
     "fst3 e |\<subseteq>| S" and "S |\<subseteq>| initials G" and "wf_dia G"
-  shows "initial_ps2 (S - fst3 e) G' = 
+  shows "initial_ps2 (S - fst3 e) G' =
   initial_ps2 S G \<ominus> fst3 e \<oplus> [ thd3 e |=> Top ]"
 proof (insert assms, unfold initial_ps2_def, transfer)
   fix G V \<Lambda> E G' V' E' e S
-  assume G_def: "G = Graph V \<Lambda> E" and G'_def: "G' = Graph V' \<Lambda> E'" and 
-    V'_def: "V' = V - fst3 e" and E'_def: "E' = removeAll e E" and 
-    e_in_E: "e \<in> set E" and fst_e_in_S: "fst3 e |\<subseteq>| S" and 
+  assume G_def: "G = Graph V \<Lambda> E" and G'_def: "G' = Graph V' \<Lambda> E'" and
+    V'_def: "V' = V - fst3 e" and E'_def: "E' = removeAll e E" and
+    e_in_E: "e \<in> set E" and fst_e_in_S: "fst3 e |\<subseteq>| S" and
     S_initials: "S |\<subseteq>| initials G" and wf_G: "wf_dia G"
   have "thd3 e |\<inter>| initials G = {||}"
     by (auto simp add: initials_def G_def e_in_E)
-  show "make_map (initials G' - (S - fst3 e)) Top ++ make_map (S - fst3 e) Bot 
-    = map_diff (make_map (initials G - S) Top ++ make_map S Bot) (fst3 e) 
-        ++ make_map (thd3 e) Top" 
+  show "make_map (initials G' - (S - fst3 e)) Top ++ make_map (S - fst3 e) Bot
+    = map_diff (make_map (initials G - S) Top ++ make_map S Bot) (fst3 e)
+        ++ make_map (thd3 e) Top"
   apply (unfold make_map_def map_diff_def)
   apply (unfold map_add_def restrict_map_def)
   apply (unfold minus_fset)
@@ -309,34 +309,34 @@ proof (insert assms, unfold initial_ps2_def, transfer)
   apply (auto simp add: fmember.rep_eq G_def e_in_E)[1]
   apply (auto simp add: fmember.rep_eq G_def e_in_E)[1]
   apply (auto simp add: fmember.rep_eq G_def e_in_E)[1]
-  apply (insert wf_G)[1] 
+  apply (insert wf_G)[1]
   apply (unfold G_def vertices.simps edges.simps)
-  apply (drule wf_dia_inv(3)) 
+  apply (drule wf_dia_inv(3))
   apply (unfold acyclicity_def)
   apply (metis fst_e_in_S inter_fset le_iff_inf set_mp)
-  apply (insert wf_G)[1] 
+  apply (insert wf_G)[1]
   apply (unfold G_def vertices.simps edges.simps)
   apply (drule wf_dia_inv(4))
   apply (drule linearityD2)
   apply (fold fset_cong, unfold inter_fset fset_simps)
   apply (insert e_in_E, blast)[1]
-  apply (insert wf_G)[1] 
+  apply (insert wf_G)[1]
   apply (unfold G_def vertices.simps edges.simps)
-  apply (drule wf_dia_inv(3)) 
-  apply (metis (lifting) e_in_E G_def empty_iff fset_simps(1) 
+  apply (drule wf_dia_inv(3))
+  apply (metis (lifting) e_in_E G_def empty_iff fset_simps(1)
     finter_iff linearityD(2) notin_fset wf_G wf_dia_inv(4))
-  apply (insert wf_G)[1] 
+  apply (insert wf_G)[1]
   apply (unfold G_def vertices.simps edges.simps)
   apply (drule wf_dia_inv(4))
   apply (drule linearityD2)
   apply (fold fset_cong, unfold inter_fset fset_simps)
   apply (insert e_in_E, blast)[1]
-  apply (insert wf_G)[1] 
+  apply (insert wf_G)[1]
   apply (unfold G_def vertices.simps edges.simps)
-  apply (drule wf_dia_inv(3)) 
-  apply (metis (lifting) e_in_E G_def empty_iff fset_simps(1) 
+  apply (drule wf_dia_inv(3))
+  apply (metis (lifting) e_in_E G_def empty_iff fset_simps(1)
     finter_iff linearityD(2) notin_fset wf_G wf_dia_inv(4))
-  apply (insert wf_G) 
+  apply (insert wf_G)
   apply (unfold G_def vertices.simps edges.simps)
   apply (drule wf_dia_inv(5))
   apply (unfold less_eq_fset.rep_eq union_fset)
@@ -362,15 +362,15 @@ proof -
   show ?thesis
   proof (intro lins2I)
     show "distinct \<pi>" using lins2D(1) by auto
-  next  
-    have "set \<pi> = set (Inl v # \<pi>) - {Inl v}" using lins2D(1) by auto 
+  next
+    have "set \<pi> = set (Inl v # \<pi>) - {Inl v}" using lins2D(1) by auto
     also have "... = (fset G^V - fset ({|v|} |\<union>| S)) <+> set G^E"
       using lins2D(2) by auto
     finally show "set \<pi> = (fset G^V - fset ({|v|} |\<union>| S)) <+> set G^E"
       by auto
   next
     fix i j v e
-    assume "i < length \<pi>" "j < length \<pi>" "\<pi> ! i = Inl v" 
+    assume "i < length \<pi>" "j < length \<pi>" "\<pi> ! i = Inl v"
       "\<pi> ! j = Inr e" "v |\<in>| fst3 e"
     thus "i < j" using lins2D(3)[of "i+1" "j+1"] by auto
   next
@@ -386,14 +386,14 @@ lemma next_lins2_edge:
       and "vs |\<subseteq>| S"
       and "e = (vs,c,ws)"
   shows "\<pi> \<in> lins2 (S - vs) (Graph (V - vs) \<Lambda> (removeAll e E))"
-proof - 
+proof -
   note lins2D = lins2D[OF assms(1)]
   show ?thesis
   proof (intro lins2I, unfold vertices.simps edges.simps)
     show "distinct \<pi>"
     using lins2D(1) by auto
   next
-    show "set \<pi> = (fset (V - vs) - fset (S - vs)) 
+    show "set \<pi> = (fset (V - vs) - fset (S - vs))
       <+> set (removeAll e E)"
     apply (insert lins2D(1) lins2D(2) assms(2))
     apply (unfold assms(3) vertices.simps edges.simps less_eq_fset.rep_eq, simp)
@@ -404,15 +404,15 @@ proof -
        fset vs \<subseteq> fset S \<longrightarrow>
        Inr (vs, c, ws) \<notin> set \<pi> \<longrightarrow>
        distinct \<pi> \<longrightarrow> (a, aa, b) \<in> set E \<longrightarrow> Inr (a, aa, b) \<notin> set \<pi> \<longrightarrow> b = ws"
-     by (metis (lifting) InrI List.set_simps(2) 
+     by (metis (lifting) InrI List.set_simps(2)
       prod.inject set_ConsD sum.simps(2))
-     
+
      moreover have "\<forall>a aa b.
        insert (Inr (vs, c, ws)) (set \<pi>) = (fset V - fset S) <+> set E \<longrightarrow>
        fset vs \<subseteq> fset S \<longrightarrow>
        Inr (vs, c, ws) \<notin> set \<pi> \<longrightarrow>
        distinct \<pi> \<longrightarrow> (a, aa, b) \<in> set E \<longrightarrow> Inr (a, aa, b) \<notin> set \<pi> \<longrightarrow> aa = c"
-     by (metis (lifting) InrI List.set_simps(2) 
+     by (metis (lifting) InrI List.set_simps(2)
       prod.inject set_ConsD sum.simps(2))
 
      moreover have "\<forall>x. insert (Inr (vs, c, ws)) (set \<pi>) = (fset V - fset S) <+> set E \<longrightarrow>
@@ -431,7 +431,7 @@ proof -
     qed
   next
     fix i j v e
-    assume "i < length \<pi>" "j < length \<pi>" "\<pi> ! i = Inl v" 
+    assume "i < length \<pi>" "j < length \<pi>" "\<pi> ! i = Inl v"
       "\<pi> ! j = Inr e" "v |\<in>| fst3 e"
     thus "i < j" using lins2D(3)[of "i+1" "j+1"] by auto
   next
@@ -444,14 +444,14 @@ qed
 
 
 text {* We wish to prove that every proofstate chain that can be obtained from
-  a linear extension of @{term G} is well-formed and has as its final 
+  a linear extension of @{term G} is well-formed and has as its final
   proofstate that state in which every terminal node in @{term G} is mapped
-  to @{term Bot}. 
-  
-  We first prove this for partially-processed diagrams, for
-  then the result for ordinary diagrams follows as an easy corollary. 
+  to @{term Bot}.
 
-  We use induction on the size of the partially-processed diagram. The size of 
+  We first prove this for partially-processed diagrams, for
+  then the result for ordinary diagrams follows as an easy corollary.
+
+  We use induction on the size of the partially-processed diagram. The size of
   a partially-processed diagram @{term "(G,S)"} is defined as the number of
   nodes in @{term G}, plus the number of edges, minus the number of nodes in
   @{term S}. *}
@@ -459,35 +459,35 @@ text {* We wish to prove that every proofstate chain that can be obtained from
 lemmas [simp] = fmember.rep_eq
 
 lemma wf_chains2:
-  fixes k 
+  fixes k
   assumes "S |\<subseteq>| initials G"
       and "wf_dia G"
       and "\<Pi> \<in> ps_chains2 S G"
       and "fcard G^V + length G^E = k + fcard S"
   shows "wf_ps_chain \<Pi> \<and> (post \<Pi> = [ terminals G |=> Bot ])"
-using assms 
+using assms
 proof (induct k arbitrary: S G \<Pi>)
   case 0
   obtain V \<Lambda> E where G_def: "G = Graph V \<Lambda> E" by (metis diagram.exhaust)
-  have "S |\<subseteq>| V" 
-    using "0.prems"(1) initials_in_vertices[of "G"] 
+  have "S |\<subseteq>| V"
+    using "0.prems"(1) initials_in_vertices[of "G"]
     by (auto simp add: G_def)
   have "fcard V \<le> fcard S"
-    using "0.prems"(4) 
+    using "0.prems"(4)
     by (unfold G_def, auto)
   from fcard_seteq[OF `S |\<subseteq>| V` this] have "S = V" by auto
   hence "E = []" using "0.prems"(4) by (unfold G_def, auto)
   have "initials G = V"
     by (unfold G_def `E=[]`, rule no_edges_imp_all_nodes_initial)
   have "terminals G = V"
-    by (unfold G_def `E=[]`, rule no_edges_imp_all_nodes_terminal)  
+    by (unfold G_def `E=[]`, rule no_edges_imp_all_nodes_terminal)
   have "{} <+> {} = {}" by auto
-  have "lins2 S G = { [] }" 
+  have "lins2 S G = { [] }"
   apply (unfold G_def `S=V` `E=[]`)
   apply (unfold lins2_def, auto simp add: `{} <+> {} = {}`)
   done
-  hence \<Pi>_def: "\<Pi> = \<lbrace> initial_ps2 S G \<rbrace>" 
-    using "0.prems"(3) 
+  hence \<Pi>_def: "\<Pi> = \<lbrace> initial_ps2 S G \<rbrace>"
+    using "0.prems"(3)
     by (auto simp add: ps_chains2_def mk_ps_chain_def)
   show ?case
   apply (intro conjI)
@@ -501,12 +501,12 @@ next
   case (Suc k)
   obtain V \<Lambda> E where G_def: "G = Graph V \<Lambda> E" by (metis diagram.exhaust)
   from Suc.prems(3) obtain \<pi> where
-    \<Pi>_def: "\<Pi> = mk_ps_chain \<lbrace> initial_ps2 S G \<rbrace> \<pi>" and 
-    \<pi>_in: "\<pi> \<in> lins2 S G" 
+    \<Pi>_def: "\<Pi> = mk_ps_chain \<lbrace> initial_ps2 S G \<rbrace> \<pi>" and
+    \<pi>_in: "\<pi> \<in> lins2 S G"
     by (auto simp add: ps_chains2_def)
   note lins2 = lins2D[OF \<pi>_in]
-  have "S |\<subseteq>| V" 
-    using Suc.prems(1) initials_in_vertices[of "G"] 
+  have "S |\<subseteq>| V"
+    using Suc.prems(1) initials_in_vertices[of "G"]
     by (auto simp add: G_def)
   show ?case
   proof (cases \<pi>)
@@ -516,7 +516,7 @@ next
     apply (unfold empty_eq_Plus_conv)
     apply (unfold G_def vertices.simps edges.simps, auto)
     by (metis `S |\<subseteq>| V` less_eq_fset.rep_eq subset_antisym)
-    
+
     with Suc.prems(4) have False by (simp add: G_def)
     thus ?thesis by auto
   next
@@ -532,16 +532,16 @@ next
       apply (simp)
       apply (subgoal_tac "Inl v \<in> (fset V - fset S) <+> set E")
       apply (metis Inl_inject Inr_not_Inl PlusE)
-      apply (metis lins2(1) lins2(2) Cons G_def Inl distinct.simps(2) 
+      apply (metis lins2(1) lins2(2) Cons G_def Inl distinct.simps(2)
         distinct_length_2_or_more edges.simps vertices.simps)
-      done  
+      done
       hence v_notin_S: "v |\<notin>| S" and v_in_V: "v |\<in>| V" by auto
-      
+
       have v_initial_not_S: "v |\<in>| initials G - S"
       apply (simp only: G_def initials_def vertices.simps edges.simps)
       apply (simp only: fminus_iff)
       apply (simp only: conj_commute, intro conjI, rule v_notin_S)
-      apply (subgoal_tac 
+      apply (subgoal_tac
         "v \<in> fset (ffilter (\<lambda>v. \<forall>e\<in>set E. v |\<notin>| thd3 e) V)")
       apply simp
       apply (simp only: filter_fset, simp, simp only: conj_commute)
@@ -553,23 +553,23 @@ next
         then have "v |\<in>| (thd3 e)" by auto
         assume "e \<in> set E"
         hence "Inr e \<in> set \<pi>" using lins2(2) by (auto simp add: G_def)
-        then obtain j where 
+        then obtain j where
           "j < length \<pi>" "0 < length \<pi>" "\<pi>!j = Inr e" "\<pi>!0 = Inl v"
         by (metis \<pi>_def x_def in_set_conv_nth length_pos_if_in_set nth_Cons_0)
         with lins2(4)[OF this `v |\<in>| (thd3 e)`] show False by auto
       qed
-      
+
       def S' \<equiv> "{|v|} |\<union>| S"
 
       def \<Pi>' \<equiv> "mk_ps_chain \<lbrace> initial_ps2 S' G \<rbrace> \<pi>'"
-      hence pre_\<Pi>': "pre \<Pi>' = initial_ps2 S' G" 
+      hence pre_\<Pi>': "pre \<Pi>' = initial_ps2 S' G"
       by (metis pre.simps(1) pre_mk_ps_chain)
 
-      def \<sigma> \<equiv> "[ initials G - ({|v|} |\<union>| S) |=> Top ] \<oplus> [ S |=> Bot ]" 
+      def \<sigma> \<equiv> "[ initials G - ({|v|} |\<union>| S) |=> Top ] \<oplus> [ S |=> Bot ]"
 
-      have "wf_ps_chain \<Pi>' \<and> (post \<Pi>' = [terminals G |=> Bot])" 
+      have "wf_ps_chain \<Pi>' \<and> (post \<Pi>' = [terminals G |=> Bot])"
       proof (intro Suc.hyps[of "S'"])
-        show "S' |\<subseteq>| initials G" 
+        show "S' |\<subseteq>| initials G"
         apply (unfold S'_def, auto)
         apply (metis fmember.rep_eq fminus_iff v_initial_not_S)
         by (metis Suc.prems(1) fmember.rep_eq fset_rev_mp)
@@ -586,9 +586,9 @@ next
         by (metis v_notin_S)
       next
         show "fcard G^V + length G^E = k + fcard S'"
-         apply (unfold S'_def) 
+         apply (unfold S'_def)
          by (auto simp add: Suc.prems(4) fcard_finsert_disjoint[OF v_notin_S])
-      qed      
+      qed
       hence
         wf_\<Pi>': "wf_ps_chain \<Pi>'" and
         post_\<Pi>': "post \<Pi>' = [terminals G |=> Bot]"
@@ -596,11 +596,11 @@ next
 
       show ?thesis
       proof (intro conjI)
-        have 1: "fdom [ {|v|} |=> Bot ] 
+        have 1: "fdom [ {|v|} |=> Bot ]
         |\<inter>| fdom ([ initials G - ({|v|} |\<union>| S) |=> Top ] \<oplus>
-     [ S |=> Bot ]) = {||}" 
-        by (metis (no_types) fdom_make_fmap fdom_union 
-          bot_least funion_iff finter_finsert_left le_iff_inf 
+     [ S |=> Bot ]) = {||}"
+        by (metis (no_types) fdom_make_fmap fmdom_add
+          bot_least funion_iff finter_finsert_left le_iff_inf
           fminus_iff finsert_fsubset sup_ge1 v_initial_not_S)
         show "wf_ps_chain \<Pi>"
         using [[unfold_abs_def = false]]
@@ -613,22 +613,22 @@ next
         apply (intro conjI)
         apply (fold wf_ps_chain_def, rule wf_\<Pi>')
         apply (intro wf_ps_triple_nodeI exI[of _ "\<sigma>"] conjI)
-        apply (unfold \<sigma>_def fdom_union fdom_make_fmap)
+        apply (unfold \<sigma>_def fmdom_add fdom_make_fmap)
         apply (metis finsertI1 fminus_iff funion_iff v_notin_S)
         apply (unfold pre_\<Pi>' initial_ps2_def S'_def)
         apply (unfold fmap_add_commute[OF 1])
-        apply (unfold fmap_add_assoc)
-        apply (fold fmap_add_assoc[of _ "[ S |=> Bot ]"])
+        apply (unfold fmadd_assoc)
+        apply (fold fmadd_assoc[of _ "[ S |=> Bot ]"])
         apply (unfold make_fmap_union sup.commute[of "{|v|}"])
         apply (unfold fminus_funion)
         using v_initial_not_S apply auto
-        by (metis (hide_lams, no_types) finsert_absorb finsert_fminus_single finter_fminus 
+        by (metis (hide_lams, no_types) finsert_absorb finsert_fminus_single finter_fminus
             inf_commute inf_idem v_initial_not_S)
       next
-        show "post \<Pi> = [ terminals G |=> Bot ]"  
+        show "post \<Pi> = [ terminals G |=> Bot ]"
         apply (unfold \<Pi>_def \<pi>_def x_def mk_ps_chain_cons, simp)
         apply (unfold mk_ps_chain_ccons post.simps)
-        apply (fold next_initial_ps2_vertex S'_def) 
+        apply (fold next_initial_ps2_vertex S'_def)
         apply (fold \<Pi>'_def, rule post_\<Pi>')
         done
       qed
@@ -642,15 +642,15 @@ next
       by (metis vs_def ws_def fst3_simp thd3_simp prod_cases3)
 
       have "linearity E" and "acyclicity E" and
-        e_in_V: "\<And>e. e \<in> set E \<Longrightarrow> fst3 e |\<union>| thd3 e |\<subseteq>| V" 
+        e_in_V: "\<And>e. e \<in> set E \<Longrightarrow> fst3 e |\<union>| thd3 e |\<subseteq>| V"
       by (insert Suc.prems(2) wf_dia_inv, unfold G_def, blast)+
       note lin = linearityD[OF this(1)]
-      
+
       have acy: "\<And>e. e \<in> set E \<Longrightarrow> fst3 e |\<inter>| thd3 e = {||}"
       apply (fold fset_cong, insert `acyclicity E`)
       apply (unfold acyclicity_def acyclic_def, auto)
       done
-      
+
       note lins = lins2D[OF \<pi>_in]
 
       have e_in_E: "e \<in> set E"
@@ -658,10 +658,10 @@ next
       apply (unfold \<pi>_def x_def G_def edges.simps, auto)[1]
       apply (simp add: lins(2))
       done
-      
+
       have vs_in_S: "vs |\<subseteq>| S"
       apply (insert e_in_V[OF e_in_E])
-      apply (unfold less_eq_fset.rep_eq) 
+      apply (unfold less_eq_fset.rep_eq)
       apply (intro subsetI)
       apply (unfold vs_def)
       apply (rule ccontr)
@@ -674,7 +674,7 @@ next
         assume "v \<notin> fset S" and "v \<in> fset V"
         hence "Inl v \<in> set \<pi>"
         by (metis (lifting) DiffI G_def InlI lins(2) vertices.simps)
-        then obtain i where 
+        then obtain i where
           "i < length \<pi>" "0 < length \<pi>" "\<pi>!i = Inl v"  "\<pi>!0 = Inr e"
         by (metis Cons Inr in_set_conv_nth length_pos_if_in_set nth_Cons_0)
         from lins(3)[OF this] show "False" by (auto simp add: a)
@@ -682,37 +682,37 @@ next
 
       have "ws |\<inter>| (initials G) = {||}"
       apply (insert e_in_V[OF e_in_E])
-      apply (unfold initials_def less_eq_fset.rep_eq fmember.rep_eq, fold fset_cong) 
+      apply (unfold initials_def less_eq_fset.rep_eq fmember.rep_eq, fold fset_cong)
       apply (unfold ws_def G_def, auto simp add: e_in_E)
       done
-      
+
       def S' \<equiv> "S - vs"
       def V' \<equiv> "V - vs"
       def E' \<equiv> "removeAll e E"
       def G' \<equiv> "Graph V' \<Lambda> E'"
 
       def \<Pi>' \<equiv> "mk_ps_chain \<lbrace> initial_ps2 S' G' \<rbrace> \<pi>'"
-      hence pre_\<Pi>': "pre \<Pi>' = initial_ps2 S' G'" 
+      hence pre_\<Pi>': "pre \<Pi>' = initial_ps2 S' G'"
       by (metis pre.simps(1) pre_mk_ps_chain)
-      
-      def \<sigma> \<equiv> "[ initials G - S |=> Top ] \<oplus> [ S - vs |=> Bot ]" 
 
-      have next_initial_ps2: "initial_ps2 S' G' 
+      def \<sigma> \<equiv> "[ initials G - S |=> Top ] \<oplus> [ S - vs |=> Bot ]"
+
+      have next_initial_ps2: "initial_ps2 S' G'
         = initial_ps2 S G \<ominus> vs \<oplus> [ws |=> Top]"
-      using next_initial_ps2_edge[OF G_def _ _ _ e_in_E _ Suc.prems(1) 
+      using next_initial_ps2_edge[OF G_def _ _ _ e_in_E _ Suc.prems(1)
         Suc.prems(2)] G'_def E'_def vs_def ws_def V'_def vs_in_S S'_def
       by auto
 
-      have "wf_ps_chain \<Pi>' \<and> post \<Pi>' = [ terminals G' |=> Bot ]" 
+      have "wf_ps_chain \<Pi>' \<and> post \<Pi>' = [ terminals G' |=> Bot ]"
       proof (intro Suc.hyps[of "S'"])
-        show "S' |\<subseteq>| initials G'" 
+        show "S' |\<subseteq>| initials G'"
         apply (insert Suc.prems(1))
         apply (unfold G'_def G_def initials_def)
         apply (unfold less_eq_fset.rep_eq S'_def E'_def V'_def)
         apply auto
         done
       next
-        from Suc.prems(2) have "wf_dia (Graph V \<Lambda> E)" 
+        from Suc.prems(2) have "wf_dia (Graph V \<Lambda> E)"
           by (unfold G_def)
         note wf_G = wf_dia_inv[OF this]
         show "wf_dia G'"
@@ -744,16 +744,16 @@ next
         apply (unfold V'_def E'_def S'_def)
         apply (unfold fcard_funion_fsubset[OF `vs |\<subseteq>| V`])
         apply (unfold fcard_funion_fsubset[OF `vs |\<subseteq>| S`])
-        apply (fold distinct_remove1_removeAll[OF `distinct E`])  
+        apply (fold distinct_remove1_removeAll[OF `distinct E`])
         apply (unfold length_remove1)
         apply (simp add: e_in_E)
         apply (drule arg_cong[of _ _ "\<lambda>x. x - fcard vs - 1"])
-        apply (subst (asm) add_diff_assoc2[symmetric]) 
+        apply (subst (asm) add_diff_assoc2[symmetric])
         apply (simp add: fcard_mono[OF `vs |\<subseteq>| V`])
         apply (subst add_diff_assoc, insert length_pos_if_in_set[OF e_in_E], arith, auto)
         apply (subst add_diff_assoc, auto simp add: fcard_mono[OF `vs |\<subseteq>| S`])
         done
-      qed      
+      qed
       hence
         wf_\<Pi>': "wf_ps_chain \<Pi>'" and
         post_\<Pi>': "post \<Pi>' = [ terminals G' |=> Bot ]"
@@ -765,10 +765,10 @@ next
       apply (fold fset_cong, auto simp add: e_in_E vs_def)
       done
 
-      have 1: "fdom [ fst3 e |=> Bot ] |\<inter>| 
-        fdom([ ffilter (\<lambda>v. \<forall>e\<in>set E. v |\<notin>| thd3 e) V - S |=> Top ] 
+      have 1: "fdom [ fst3 e |=> Bot ] |\<inter>|
+        fdom([ ffilter (\<lambda>v. \<forall>e\<in>set E. v |\<notin>| thd3 e) V - S |=> Top ]
         \<oplus> [ S - fst3 e |=> Bot ]) = {||}"
-      apply (unfold fdom_union fdom_make_fmap)
+      apply (unfold fmdom_add fdom_make_fmap)
       apply (fold fset_cong)
       apply auto
       apply (metis in_mono less_eq_fset.rep_eq vs_def vs_in_S)
@@ -788,32 +788,32 @@ next
         apply (intro conjI)
         apply (fold wf_ps_chain_def)
         apply (rule wf_\<Pi>')
-        apply (intro wf_ps_triple_edgeI exI[of _ "\<sigma>"]) 
+        apply (intro wf_ps_triple_edgeI exI[of _ "\<sigma>"])
         apply (unfold e_def fst3_simp thd3_simp \<sigma>_def, intro conjI)
         apply (insert Suc.prems(1))
         apply (unfold pre_\<Pi>' initial_ps2_def initials_def)
         apply (insert vs_in_S acy[OF e_in_E])
         apply (fold fset_cong)
-        apply (unfold less_eq_fset.rep_eq)[1] 
+        apply (unfold less_eq_fset.rep_eq)[1]
         apply (unfold G_def G'_def vs_def ws_def V'_def E'_def S'_def)
         apply (unfold vertices.simps edges.simps)
         apply (unfold fmap_add_commute[OF 1])
-        apply (fold fmap_add_assoc)
+        apply (fold fmadd_assoc)
         apply (unfold make_fmap_union)
-        apply (auto simp add: fdom_union fdom_make_fmap e_in_E)[1]
+        apply (auto simp add: fdom_make_fmap e_in_E)[1]
         apply simp
-        apply (unfold fmap_add_assoc)
-        apply (unfold make_fmap_union)  
+        apply (unfold fmadd_assoc)
+        apply (unfold make_fmap_union)
         apply (metis (lifting) funion_absorb2 vs_def vs_in_S)
-        apply (intro arg_cong2[of _ _ "[ S - fst3 e |=> Bot ]" 
+        apply (intro arg_cong2[of _ _ "[ S - fst3 e |=> Bot ]"
             "[ S - fst3 e |=> Bot ]" "op \<oplus>"])
         apply (intro arg_cong2[of _ _ "Top" "Top" "make_fmap"])
         defer 1
-        apply (simp, simp)       
+        apply (simp, simp)
         apply (fold fset_cong)
         apply (unfold less_eq_fset.rep_eq fmember.rep_eq, simp)
         apply (elim conjE)
-        apply (intro set_eqI iffI, simp_all) 
+        apply (intro set_eqI iffI, simp_all)
         apply (elim conjE, intro disjI conjI ballI, simp)
         apply (case_tac "ea=e", simp_all)
         apply (elim disjE conjE, intro conjI ballI impI, simp_all)
@@ -826,7 +826,7 @@ next
         apply blast
         apply (metis G_def Suc(3) e_in_E set_mp less_eq_fset.rep_eq wf_dia_inv')
         prefer 2
-        apply (metis (lifting) IntI Suc(2) `ws |\<inter>| initials G = {||}` 
+        apply (metis (lifting) IntI Suc(2) `ws |\<inter>| initials G = {||}`
             empty_iff fset_simps(1) in_mono inter_fset less_eq_fset.rep_eq ws_def)
         apply auto
         done
@@ -846,11 +846,11 @@ next
   qed
 qed
 
-corollary wf_chains:  
+corollary wf_chains:
   assumes "wf_dia G"
   assumes "\<Pi> \<in> ps_chains G"
   shows "wf_ps_chain \<Pi> \<and> post \<Pi> = [ terminals G |=> Bot ]"
-apply (intro wf_chains2[of "{||}"], insert assms(2)) 
+apply (intro wf_chains2[of "{||}"], insert assms(2))
 by (auto simp add: assms(1) ps_chains_is_ps_chains2_with_empty_S fcard_fempty)
 
 
@@ -861,21 +861,21 @@ type_synonym int_chain = "(interface, assertion_gadget + command_gadget) chain"
 text {* An interface chain is similar to a proofstate chain. However, where a
   proofstate chain talks about nodes and edges, an interface chain talks about
   the assertion-gadgets and command-gadgets that label those nodes and edges
-  in a diagram. And where a proofstate chain talks about proofstates, an 
-  interface chain talks about the interfaces obtained from those proofstates. 
+  in a diagram. And where a proofstate chain talks about proofstates, an
+  interface chain talks about the interfaces obtained from those proofstates.
 
-  The following functions convert a proofstate chain into an 
+  The following functions convert a proofstate chain into an
   interface chain. *}
 
 definition
   ps_to_int :: "[diagram, proofstate] \<Rightarrow> interface"
 where
-  "ps_to_int G \<sigma> \<equiv> 
+  "ps_to_int G \<sigma> \<equiv>
     \<Otimes>v |\<in>| fdom \<sigma>. case_topbot top_ass bot_ass (lookup \<sigma> v) (G^\<Lambda> v)"
 
 definition
   ps_chain_to_int_chain :: "[diagram, ps_chain] \<Rightarrow> int_chain"
-where 
+where
   "ps_chain_to_int_chain G \<Pi> \<equiv>
     chainmap (ps_to_int G) ((case_sum (Inl \<circ> G^\<Lambda>) (Inr \<circ> snd3))) \<Pi>"
 
@@ -886,40 +886,40 @@ by (simp add: ps_chain_to_int_chain_def)
 
 subsection {* Soundness proof *}
 
-text {*  We assume that @{term wr_com} always returns @{term "{}"}. This is 
-  equivalent to changing our axiomatization of separation logic such that the 
+text {*  We assume that @{term wr_com} always returns @{term "{}"}. This is
+  equivalent to changing our axiomatization of separation logic such that the
   frame rule has no side-condition. One way to obtain a separation logic
   lacking a side-condition on its frame rule is to use variables-as-
   resource.
 
   We proceed by induction on the proof rules for graphical diagrams. We
-  show that: (1) if a diagram @{term G} is provable w.r.t. interfaces 
-  @{term P} and @{term Q}, then @{term P} and @{term Q} are the top and bottom 
+  show that: (1) if a diagram @{term G} is provable w.r.t. interfaces
+  @{term P} and @{term Q}, then @{term P} and @{term Q} are the top and bottom
   interfaces of @{term G}, and that the Hoare triple @{term "(asn P,
   c, asn Q)"} is provable for each command @{term c} that can be extracted
-  from @{term G}; (2) if a command-gadget @{term C} is provable w.r.t. 
+  from @{term G}; (2) if a command-gadget @{term C} is provable w.r.t.
   interfaces @{term P} and @{term Q}, then the Hoare triple @{term "(asn P,
   c, asn Q)"} is provable for each command @{term c} that can be extracted
   from @{term C}; and (3) if an assertion-gadget @{term A} is provable, and if
-  the top and bottom interfaces of @{term A} are @{term P} and @{term Q} 
-  respectively, then the Hoare triple @{term "(asn P, c, asn Q)"} is provable 
+  the top and bottom interfaces of @{term A} are @{term P} and @{term Q}
+  respectively, then the Hoare triple @{term "(asn P, c, asn Q)"} is provable
   for each command @{term c} that can be extracted from @{term A}. *}
 
 
 
 lemma soundness_graphical_helper:
   assumes no_var_interference: "\<And>c. wr_com c = {}"
-  shows 
-    "(prov_dia G P Q \<longrightarrow> 
-      (P = top_dia G \<and> Q = bot_dia G \<and> 
-      (\<forall>c. coms_dia G c \<longrightarrow> prov_triple (asn P, c, asn Q)))) 
-   \<and> (prov_com C P Q \<longrightarrow> 
+  shows
+    "(prov_dia G P Q \<longrightarrow>
+      (P = top_dia G \<and> Q = bot_dia G \<and>
+      (\<forall>c. coms_dia G c \<longrightarrow> prov_triple (asn P, c, asn Q))))
+   \<and> (prov_com C P Q \<longrightarrow>
       (\<forall>c. coms_com C c \<longrightarrow> prov_triple (asn P, c, asn Q)))
-   \<and> (prov_ass A \<longrightarrow> 
+   \<and> (prov_ass A \<longrightarrow>
       (\<forall>c. coms_ass A c \<longrightarrow> prov_triple (asn (top_ass A), c, asn (bot_ass A))))"
 proof (induct rule: prov_dia_prov_com_prov_ass.induct)
   case (Skip p)
-  thus ?case 
+  thus ?case
   apply (intro allI impI, elim conjE coms_skip_inv)
   apply (auto simp add: prov_triple.skip)
   done
@@ -948,30 +948,30 @@ next
 next
   case (Main G)
   thus ?case
-  apply (intro conjI) 
+  apply (intro conjI)
   apply (simp, simp)
   apply (intro allI impI)
   apply (elim coms_main_inv, simp)
   proof -
-    fix c V \<Lambda> E 
+    fix c V \<Lambda> E
     fix \<pi>::"lin"
     fix cs::"command list"
     assume wf_G: "wf_dia (Graph V \<Lambda> E)"
-    assume "\<And>v. v \<in> fset V \<Longrightarrow> \<forall>c. coms_ass (\<Lambda> v) c \<longrightarrow> 
+    assume "\<And>v. v \<in> fset V \<Longrightarrow> \<forall>c. coms_ass (\<Lambda> v) c \<longrightarrow>
       prov_triple (asn (top_ass (\<Lambda> v)), c, asn (bot_ass (\<Lambda> v)))"
-    hence prov_vertex: "\<And>v c P Q F. \<lbrakk> coms_ass (\<Lambda> v) c; v \<in> fset V; 
-      P = (top_ass (\<Lambda> v) \<otimes> F) ; Q = (bot_ass (\<Lambda> v) \<otimes> F) \<rbrakk> 
-      \<Longrightarrow> prov_triple (asn P, c, asn Q)" 
+    hence prov_vertex: "\<And>v c P Q F. \<lbrakk> coms_ass (\<Lambda> v) c; v \<in> fset V;
+      P = (top_ass (\<Lambda> v) \<otimes> F) ; Q = (bot_ass (\<Lambda> v) \<otimes> F) \<rbrakk>
+      \<Longrightarrow> prov_triple (asn P, c, asn Q)"
     by (auto simp add: prov_triple.frame no_var_interference)
-    assume "\<And>e. e \<in> set E \<Longrightarrow> \<forall>c. coms_com (snd3 e) c \<longrightarrow> prov_triple 
+    assume "\<And>e. e \<in> set E \<Longrightarrow> \<forall>c. coms_com (snd3 e) c \<longrightarrow> prov_triple
       (asn (\<Otimes>v|\<in>|fst3 e. bot_ass (\<Lambda> v)),c,asn (\<Otimes>v|\<in>|thd3 e. top_ass (\<Lambda> v)))"
-    hence prov_edge: "\<And>e c P Q F. \<lbrakk> e \<in> set E ; coms_com (snd3 e) c ; 
+    hence prov_edge: "\<And>e c P Q F. \<lbrakk> e \<in> set E ; coms_com (snd3 e) c ;
       P = ((\<Otimes>v|\<in>|fst3 e. bot_ass (\<Lambda> v)) \<otimes> F) ;
-      Q = ((\<Otimes>v|\<in>|thd3 e. top_ass (\<Lambda> v)) \<otimes> F) \<rbrakk> 
+      Q = ((\<Otimes>v|\<in>|thd3 e. top_ass (\<Lambda> v)) \<otimes> F) \<rbrakk>
       \<Longrightarrow> prov_triple (asn P, c, asn Q)"
     by (auto simp add: prov_triple.frame no_var_interference)
     assume len_cs: "length cs = length \<pi>"
-    assume "\<forall>i<length \<pi>. 
+    assume "\<forall>i<length \<pi>.
       case_sum (coms_ass \<circ> \<Lambda>) (coms_com \<circ> snd3) (\<pi> ! i) (cs ! i)"
     hence \<pi>_cs: "\<And>i. i < length \<pi> \<Longrightarrow>
       case_sum (coms_ass \<circ> \<Lambda>) (coms_com \<circ> snd3) (\<pi> ! i) (cs ! i)" by auto
@@ -980,15 +980,15 @@ next
     assume \<pi>_lin: "\<pi> \<in> lins (Graph V \<Lambda> E)"
 
     note lins = linsD[OF \<pi>_lin]
-    
+
     def \<Pi> \<equiv> "mk_ps_chain \<lbrace> initial_ps G \<rbrace> \<pi>"
-    
+
     have "\<Pi> \<in> ps_chains G" by (simp add: \<pi>_lin \<Pi>_def ps_chains_def G_def)
     hence 1: "post \<Pi> = [ terminals G |=> Bot ]"
       and 2: "chain_all wf_ps_triple \<Pi>"
     by (insert wf_chains G_def wf_G, auto simp add: wf_ps_chain_def)
-    
-    show "prov_triple (asn (\<Otimes>v|\<in>|initials (Graph V \<Lambda> E). top_ass (\<Lambda> v)), 
+
+    show "prov_triple (asn (\<Otimes>v|\<in>|initials (Graph V \<Lambda> E). top_ass (\<Lambda> v)),
       foldr op ;; cs Skip, asn (\<Otimes>v|\<in>|terminals (Graph V \<Lambda> E). bot_ass (\<Lambda> v)))"
     using [[unfold_abs_def = false]]
     apply (intro seq_fold[of _ "ps_chain_to_int_chain G \<Pi>"])
@@ -1002,11 +1002,11 @@ next
     apply (unfold ps_to_int_def)
     apply (unfold fdom_make_fmap)
     apply (unfold G_def labelling.simps, fold G_def)
-    apply (subgoal_tac "\<forall>v \<in> fset (initials G). top_ass (\<Lambda> v) = 
+    apply (subgoal_tac "\<forall>v \<in> fset (initials G). top_ass (\<Lambda> v) =
       case_topbot top_ass bot_ass (lookup [ initials G |=> Top ] v) (\<Lambda> v)")
     apply (unfold iter_hcomp_cong, simp)
     apply (metis lookup_make_fmap topbot.simps(3))
-    apply (subgoal_tac "\<forall>v \<in> fset (terminals G). bot_ass (\<Lambda> v) = 
+    apply (subgoal_tac "\<forall>v \<in> fset (terminals G). bot_ass (\<Lambda> v) =
       case_topbot top_ass bot_ass (lookup [ terminals G |=> Bot ] v) (\<Lambda> v)")
     apply (unfold iter_hcomp_cong, simp)
     apply (metis lookup_make_fmap topbot.simps(4), simp)
@@ -1015,11 +1015,11 @@ next
       fix i
       assume "i < length \<pi>"
       hence "i < chainlen \<Pi>"
-      by (metis \<Pi>_def add_0_left chainlen.simps(1) 
+      by (metis \<Pi>_def add_0_left chainlen.simps(1)
         mk_ps_chain_preserves_length)
-      hence wf_\<Pi>i: "wf_ps_triple (nthtriple \<Pi> i)" 
+      hence wf_\<Pi>i: "wf_ps_triple (nthtriple \<Pi> i)"
         by (insert 2, simp add: chain_all_nthtriple)
-      show "prov_triple (asn (fst3 (nthtriple (ps_chain_to_int_chain G \<Pi>) i)), 
+      show "prov_triple (asn (fst3 (nthtriple (ps_chain_to_int_chain G \<Pi>) i)),
                  cs ! i, asn (thd3 (nthtriple (ps_chain_to_int_chain G \<Pi>) i)))"
       apply (unfold ps_chain_to_int_chain_def)
       apply (unfold nthtriple_chainmap[OF `i < chainlen \<Pi>`])
@@ -1032,27 +1032,27 @@ next
         apply (auto simp add: \<Pi>_def comlist_mk_ps_chain Inl)
         done
 
-        with wf_\<Pi>i wf_ps_triple_def obtain \<sigma> where 
+        with wf_\<Pi>i wf_ps_triple_def obtain \<sigma> where
           v_notin_\<sigma>: "v |\<notin>| fdom \<sigma>" and
           fst_\<Pi>i: "fst3 (nthtriple \<Pi> i) = [ {|v|} |=> Top ] \<oplus> \<sigma>" and
           thd_\<Pi>i: "thd3 (nthtriple \<Pi> i) = [ {|v|} |=> Bot ] \<oplus> \<sigma>" by auto
 
-        show "prov_triple (asn (ps_to_int G (fst3 (nthtriple \<Pi> i))), 
+        show "prov_triple (asn (ps_to_int G (fst3 (nthtriple \<Pi> i))),
                    cs ! i, asn (ps_to_int G (thd3 (nthtriple \<Pi> i))))"
         apply (intro prov_vertex[where v=v])
         apply (metis (no_types) Inl `i < length \<pi>` \<pi>_cs o_def sum.simps(5))
-        apply (metis (lifting) Inl lins(2) Inl_not_Inr PlusE `i < length \<pi>` 
+        apply (metis (lifting) Inl lins(2) Inl_not_Inr PlusE `i < length \<pi>`
           nth_mem sum.simps(1) vertices.simps)
         apply (unfold fst_\<Pi>i thd_\<Pi>i)
         apply (unfold ps_to_int_def)
-        apply (unfold fdom_union fdom_make_fmap)
+        apply (unfold fmdom_add fdom_make_fmap)
         apply (unfold finsert_is_funion[symmetric])
         apply (insert v_notin_\<sigma>)
         apply (unfold iter_hcomp_insert)
         apply (unfold lookup_union2 lookup_make_fmap1)
         apply (unfold G_def labelling.simps)
-        apply (subgoal_tac "\<forall>va \<in> fset (fdom \<sigma>). case_topbot top_ass bot_ass 
-          (lookup ([ {|v|} |=> Top ] \<oplus> \<sigma>) va) (\<Lambda> va) = 
+        apply (subgoal_tac "\<forall>va \<in> fset (fdom \<sigma>). case_topbot top_ass bot_ass
+          (lookup ([ {|v|} |=> Top ] \<oplus> \<sigma>) va) (\<Lambda> va) =
           case_topbot top_ass bot_ass (lookup ([{|v|} |=> Bot] \<oplus> \<sigma>) va)(\<Lambda> va)")
         apply (unfold iter_hcomp_cong, simp)
         apply (metis fmember.rep_eq lookup_union1, simp)
@@ -1068,10 +1068,10 @@ next
           fst_e_disjoint_\<sigma>: "fst3 e |\<inter>| fdom \<sigma> = {||}" and
           thd_e_disjoint_\<sigma>: "thd3 e |\<inter>| fdom \<sigma> = {||}" and
           fst_\<Pi>i: "fst3 (nthtriple \<Pi> i) = [ fst3 e |=> Bot ] \<oplus> \<sigma>" and
-          thd_\<Pi>i: "thd3 (nthtriple \<Pi> i) = [ thd3 e |=> Top ] \<oplus> \<sigma>" 
+          thd_\<Pi>i: "thd3 (nthtriple \<Pi> i) = [ thd3 e |=> Top ] \<oplus> \<sigma>"
         by (auto simp add: inf_sup_distrib2)
 
-        show "prov_triple (asn (ps_to_int G (fst3 (nthtriple \<Pi> i))), 
+        show "prov_triple (asn (ps_to_int G (fst3 (nthtriple \<Pi> i))),
                    cs ! i, asn (ps_to_int G (thd3 (nthtriple \<Pi> i))))"
         apply (intro prov_edge[where e=e])
         apply (subgoal_tac "Inr e \<in> set \<pi>")
@@ -1081,10 +1081,10 @@ next
         apply (unfold fst_\<Pi>i thd_\<Pi>i)
         apply (unfold ps_to_int_def)
         apply (unfold G_def labelling.simps)
-        apply (unfold fdom_union fdom_make_fmap)
+        apply (unfold fmdom_add fdom_make_fmap)
         apply (insert fst_e_disjoint_\<sigma>)
         apply (unfold iter_hcomp_union)
-        apply (subgoal_tac "\<forall>v \<in> fset (fst3 e). case_topbot top_ass bot_ass 
+        apply (subgoal_tac "\<forall>v \<in> fset (fst3 e). case_topbot top_ass bot_ass
           (lookup ([ fst3 e |=> Bot ] \<oplus> \<sigma>) v) (\<Lambda> v) = bot_ass (\<Lambda> v)")
         apply (unfold iter_hcomp_cong)
         apply (simp)
@@ -1095,11 +1095,11 @@ next
         apply (metis fempty_iff finterI fmember.rep_eq)
         apply (insert thd_e_disjoint_\<sigma>)
         apply (unfold iter_hcomp_union)
-        apply (subgoal_tac "\<forall>v \<in> fset (thd3 e). case_topbot top_ass bot_ass 
+        apply (subgoal_tac "\<forall>v \<in> fset (thd3 e). case_topbot top_ass bot_ass
           (lookup ([ thd3 e |=> Top ] \<oplus> \<sigma>) v) (\<Lambda> v) = top_ass (\<Lambda> v)")
         apply (unfold iter_hcomp_cong)
-        apply (subgoal_tac "\<forall>v \<in> fset (fdom \<sigma>). case_topbot top_ass bot_ass 
-          (lookup ([ thd3 e |=> Top ] \<oplus> \<sigma>) v) (\<Lambda> v) = 
+        apply (subgoal_tac "\<forall>v \<in> fset (fdom \<sigma>). case_topbot top_ass bot_ass
+          (lookup ([ thd3 e |=> Top ] \<oplus> \<sigma>) v) (\<Lambda> v) =
           case_topbot top_ass bot_ass (lookup ([fst3 e |=> Bot] \<oplus> \<sigma>) v) (\<Lambda> v)")
         apply (unfold iter_hcomp_cong)
         apply simp
